\documentclass{article}
\usepackage{graphicx}
\usepackage{amsmath}
\usepackage{hyperref}
\usepackage{epigraph} 

\title{Linear Algebra Done Right\\Solutions to Exercises 1.A}
\author{}
\date{}

\begin{document}

\maketitle

\section{Inverse of a complex number}
\subsection*{Problem statement}
Suppose $a$ and $b$ are real numbers, not both $0$. Find real numbers $c$ and $d$ such that 
\[1/(a+bi)=c+di\]

\subsection*{Solution}
While we weren't given the definition of the complex conjugate\footnote{We'll have to wait for Chapter 4 to get Definition 4.3.} in Chapter 1.A, we can find $c$ and $d$ by multiplying $1/(a+bi)$ by its complex conjugate. 
Hence we have
\begin{equation*}
    \frac{1}{a+bi}\frac{a-bi}{a-bi}=\frac{a-bi}{(a^2+b^2)+(-ab+ab)i}=\frac{a-bi}{a^2+b^2}=\frac{a}{a^2+b^2}+\frac{-b}{a^2+b^2}i
\end{equation*}
where the first equality comes from the definition of addition and multiplication on $\textbf{C}$ (Definition 1.1). Thus $c=a/(a^2+b^2)$ and $d=-b/(a^2+b^2)$.

\clearpage

\section{Cube root of $1$}
\subsection*{Problem statement}
Show that 
\[\frac{-1+\sqrt{3}i}{2}\]
is a cube root of $1$ (meaning that is cube equals $1$).

\subsection*{Solution}
\begin{align*}
    \left( \frac{-1+\sqrt{3}i}{2}\right)^3&=\left( \frac{-1+\sqrt{3}i}{2}\right)\left( \frac{-1+\sqrt{3}i}{2}\right) \left( \frac{-1+\sqrt{3}i}{2} \right)\\
    &=\frac{1}{8}(-1+\sqrt{3}i)(-1+\sqrt{3}i)(-1+\sqrt{3}i)\\
    &=\frac{1}{8}((1-3)+(-2\sqrt{3})i)(-1+\sqrt{3}i)\\
    &=\frac{1}{8}(-2-2\sqrt{3}i)(-1+\sqrt{3}i)\\
    &=\frac{1}{8}((2+6)+(-2\sqrt{3}+2\sqrt{3})i)\\
    &=\frac{1}{8}(8+0i)\\
    &=1
\end{align*}

\clearpage

\section{Square roots of $i$}
\subsection*{Problem statement}
Find two distinct square roots of $i$.

\subsection*{Solution}
The square roots of $i$ concern $\frac{1}{\sqrt{2}}$.

\begin{align*}
    (\frac{1}{\sqrt{2}}+\frac{1}{\sqrt{2}}i)^2&=(\frac{1}{\sqrt{2}}+\frac{1}{\sqrt{2}}i)(\frac{1}{\sqrt{2}}+\frac{1}{\sqrt{2}}i)\\
    &=(\frac{1}{2}-\frac{1}{2})+(\frac{1}{2}+\frac{1}{2})i\\
    &=0+1i\\
    &=i
\end{align*}

\begin{align*}
    (-\frac{1}{\sqrt{2}}-\frac{1}{\sqrt{2}}i)^2&=(-\frac{1}{\sqrt{2}}-\frac{1}{\sqrt{2}}i)(-\frac{1}{\sqrt{2}}-\frac{1}{\sqrt{2}}i)\\
    &=(\frac{1}{2}-\frac{1}{2})+(\frac{1}{2}+\frac{1}{2})i\\
    &=0+1i\\
    &=i
\end{align*}


\end{document}